src/impl/TLS13.Impl.Client.fsti
@@ -154,7 +154,9 @@ let client_state_ref (c:client) : CR.state_ref =
 fn new_client_default ()
   returns c:client
   ensures CR.connection_exactly c CR.default_initial_state **
-          pure (CT.client_state_correct CR.default_initial_state)
+          pure (CT.client_state_correct CR.default_initial_state /\
+                CS.connection_state_sent_seal_replay_consistent
+                  CR.default_initial_state)
 
 fn new_client
   (server_name:array U8.t)
@@ -181,7 +183,12 @@ fn new_client
             (CR.configured_initial_state
               (Ghost.reveal 'server_name_bytes)
               (Ghost.reveal 'trust_anchors_bytes)
-              validation_time_seconds))
+              validation_time_seconds) /\
+                CS.connection_state_sent_seal_replay_consistent
+                  (CR.configured_initial_state
+                    (Ghost.reveal 'server_name_bytes)
+                    (Ghost.reveal 'trust_anchors_bytes)
+                    validation_time_seconds))
 
 fn control_snapshot
   (c:client)
